proof/spec/XMSS_vs_XMSS_MT.ec
@@ -1,0 +1,56 @@
+from Jasmin require import JModel.
+require import XMSS_PRF XMSS_MT_PRF IntDiv Params Int Ring Address Array8.
+import IntID.
+
+equiv keygen : XMSS_PRF.kg ~ XMSS_MT_PRF.kg : d = 1 ==> ={res}. 
+proof. 
+proc; inline *; sim.
+by auto => /> /#. 
+qed.
+
+equiv sign : XMSS_PRF.sign ~ XMSS_MT_PRF.sign : d=1 /\ h < 32 /\ 0 < to_uint sk{2}.`Types.idx < 2^h - 1 /\ ={arg} ==> ={res}. 
+proof. 
+proc. 
+rcondf {2} 24.
++ move => ?.
+  wp;call(:true);1:by trivial.
+  wp;call(:true);1:by trivial.
+  by auto => /> /#.
+wp;call(: true); 1: by sim.
+wp;call(: true); 1: by sim.
+auto => /> &2 => ->; rewrite !divz1 /=.
+move => *; do split.
++ rewrite W32.and_mod /=;1:smt(ge0_h).
+  by rewrite modz_small /=; 1:smt().
+
+rewrite to_uint_shr;1:smt(ge0_h).
+rewrite /zero_address /set_tree_addr /set_layer_addr /=.
+have -> : (to_uint sk{2}.`Types.idx %/ 2 ^ h) = 0 by smt().
+apply tP => i ib.
+rewrite !initiE 1:/# /=.
+rewrite !get_setE 1..3:/#.
+by rewrite initiE 1:/# /=.
+
+qed.
+
+equiv verify : XMSS_PRF.verify ~ XMSS_MT_PRF.verify : d=1 /\ h < 32 /\ 0 < to_uint s{2}.`Types.sig_idx < 2^h - 1 /\ ={arg} ==> ={res}. 
+proof. 
+proc. 
+rcondf {2} 16.
++ move => ?.
+  wp;call(:true);1:by trivial.
+  by auto => /> /#.
+wp;call(: true); 1: by sim.
+auto => /> &2 => ->; rewrite !divz1 /=.
+move => *; do split.
++ rewrite W32.and_mod /=;1:smt(ge0_h).
+  by rewrite modz_small /=; 1:smt().
+
+rewrite to_uint_shr;1:smt(ge0_h).
+rewrite /zero_address /set_tree_addr /set_layer_addr /=.
+have -> : (to_uint s{2}.`Types.sig_idx %/ 2 ^ h) = 0 by smt().
+apply tP => i ib.
+rewrite !initiE 1:/# /=.
+rewrite !get_setE 1..3:/#.
+by rewrite initiE 1:/# /=.
+qed.
